src/Syntax.v
@@ -232,7 +232,7 @@ Section System.
   Definition rulesOf := sys_rules.
 
   Definition handlersOf (rules: list Rule): list MsgId :=
-    concat (map rule_mids rules).
+    List.concat (map rule_mids rules).
 
   Definition extHandlersOf (sys: System): list MsgId :=
     filter (fun mid => isExternal sys (mid_from mid))
